AlphaCentauri.lean
@@ -59,6 +59,7 @@ public import AlphaCentauri.ToFoundation.Fvar
 public import AlphaCentauri.ToFoundation.Hierarchy
 public import AlphaCentauri.ToFoundation.Primrec
 public import AlphaCentauri.ToFoundation.Rew
+public import AlphaCentauri.ToFoundation.Schemata
 public import AlphaCentauri.ToFoundation.Semiformula
 public import AlphaCentauri.ToFoundation.Theory
 public import AlphaCentauri.ToMathlib.Goodstein
