AlphaCentauri/ToFoundation/Rew.lean
@@ -66,6 +66,14 @@ lemma subst_subst_eq {m : ℕ} (v : Fin n → Semiterm L ξ m) (φ : Semiformula
       | succ i => exact i.elim0
     · simp [Rew.comp_app]
 
+@[simp] lemma subst_bShift_eq (v : Fin 1 → Semiterm L ξ 1) (t : Semiterm L ξ 0) :
+    Rew.subst v (Rew.bShift t) = Rew.bShift t := by
+  have e : (Rew.subst v).comp (Rew.bShift : Rew L ξ 0 ξ 1) = Rew.bShift := by
+    ext x
+    · exact x.elim0
+    · simp [Rew.comp_app]
+  simpa [Rew.comp_app] using Rew.ext' e t
+
 lemma shift_subst_eq (φ : Semiformula L ℕ 1) (t : SyntacticSemiterm L n) :
     Rew.shift ▹ (φ/[t]) = (Rew.shift ▹ φ)/[Rew.shift t] := by
   simpa [← TransitiveRewriting.comp_app] using Rewriting.smul_ext' <| by
@@ -90,18 +98,20 @@ lemma rewriteMap_subst_eq_free (φ : Semiformula L ℕ 1) (h : ¬φ.FVar? m) :
   exact Semiformula.rew_eq_of_funEqOn (by simp [Rew.comp_app])
     fun x hx ↦ by simp [Rew.comp_app, ne_of_mem_of_not_mem hx h]
 
-/-- Renaming a variable that none of the formulas mentions to the new bound variable shifts the
-multiset. -/
+/-- Renaming a variable that the formula avoids to the new bound variable shifts the formula. -/
+lemma rewriteMap_eq_shift {n} (φ : Semiformula L ℕ n) (h : ¬φ.FVar? m) :
+    (@Rew.rewriteMap L ℕ ℕ n fun x ↦ if x = m then 0 else x + 1) ▹ φ = Rewriting.shift φ := by
+  have e : (@Rew.rewriteMap L ℕ ℕ n fun x ↦ if x = m then 0 else x + 1) ▹ φ =
+      (Rew.shift : SyntacticRew L n n) ▹ φ :=
+    Semiformula.rew_eq_of_funEqOn (by simp) (by
+      intro x hx
+      simp [ne_of_mem_of_not_mem hx h])
+  simpa [Rewriting.shift] using e
+
+/-- Renaming a variable that none of the formulas mentions shifts the multiset. -/
 lemma map_rewriteMap_eq_shifts (Γ : Multiset (Semiformula L ℕ 0))
     (h : ∀ φ ∈ Γ, ¬φ.FVar? m) :
-    Γ.map (fun φ ↦ (@Rew.rewriteMap L ℕ ℕ 0 fun x ↦ if x = m then 0 else x + 1) ▹ φ) = Γ⁺ := by
-  apply Multiset.map_congr rfl
-  intro φ hφ
-  have e : (@Rew.rewriteMap L ℕ ℕ 0 fun x ↦ if x = m then 0 else x + 1) ▹ φ =
-      (Rew.shift : SyntacticRew L 0 0) ▹ φ :=
-    Semiformula.rew_eq_of_funEqOn₀ (by
-      intro x hx
-      simp [ne_of_mem_of_not_mem hx (h φ hφ)])
-  simpa [Rewriting.shift] using e
+    Γ.map (fun φ ↦ (@Rew.rewriteMap L ℕ ℕ 0 fun x ↦ if x = m then 0 else x + 1) ▹ φ) = Γ⁺ :=
+  Multiset.map_congr rfl fun φ hφ ↦ rewriteMap_eq_shift φ (h φ hφ)
 
 end FFL.FirstOrder.Semiformula
